WIP inductive predicates for wstep of comp_op

nondeterministic_dataflow/Wstep_Composition.thy
@@ -4,7 +4,6 @@ imports
   "BNA_Operators"
 begin
 
-
 inductive wstep_comp_op where
   \<open>comp_op wire buf' op1' op2' = comp_op wire buf op1 op2 \<Longrightarrow> wstep_comp_op Tau wire buf buf' op1 op1' op2 op2'\<close>
 | \<open>step Tau op1 op1' \<Longrightarrow> wstep_comp_op Tau wire buf buf' op1' op1'' op2 op2' \<Longrightarrow> wstep_comp_op Tau wire buf buf' op1 op1'' op2 op2'\<close>
@@ -241,43 +240,5 @@ lemma wstep_comp_op:
       by blast
     done
   done
-
-inductive wstep_comp_op_L where
-  \<open>io = Tau \<Longrightarrow> buf = (\<lambda>_. []) \<Longrightarrow> op' = op \<Longrightarrow> wstep_comp_op_L io wire buf op op'\<close>
-| \<open>io = Inp (Inl p) x \<Longrightarrow> step (Inp p x) op op' \<Longrightarrow> wstep_comp_op_L Tau wire buf op' op'' \<Longrightarrow>
-  wstep_comp_op_L io wire buf op op''\<close>
-| \<open>io = Out (Inl p) x \<Longrightarrow> step (Out p x) op op' \<Longrightarrow> p \<notin> dom wire \<Longrightarrow>
-  wstep_comp_op_L Tau wire buf op' op'' \<Longrightarrow> wstep_comp_op_L io wire buf op op''\<close>
-| \<open>step (Out p x) op op' \<Longrightarrow> p \<in> dom wire \<Longrightarrow> wstep_comp_op_L io wire buf op' op'' \<Longrightarrow>
-  buf' = BENQ p x buf \<Longrightarrow> wstep_comp_op_L io wire buf' op op''\<close>
-| \<open>step Tau op op' \<Longrightarrow> wstep_comp_op_L io wire buf op' op'' \<Longrightarrow> wstep_comp_op_L io wire buf op op''\<close>
-
-inductive wstep_comp_op_R where
-  \<open>io = Tau \<Longrightarrow> op' = op \<Longrightarrow> wstep_comp_op_R io wire buf op op'\<close>
-| \<open>io = Inp (Inr p) x \<Longrightarrow> step (Inp p x) op op' \<Longrightarrow> p \<notin> ran wire \<Longrightarrow>
-  wstep_comp_op_R Tau wire buf op' op'' \<Longrightarrow> wstep_comp_op_R io wire buf op op''\<close>
-| \<open>step (Inp p x) op op' \<Longrightarrow> p \<in> ran wire \<Longrightarrow> wstep_comp_op_R io wire buf op' op'' \<Longrightarrow>
-  buf p \<noteq> [] \<Longrightarrow> x = BHD p buf \<Longrightarrow> buf' = BTL p buf \<Longrightarrow> wstep_comp_op_R io wire buf' op op''\<close>
-| \<open>io = Out (Inr p) x \<Longrightarrow> step (Out p x) op op' \<Longrightarrow> wstep_comp_op_R Tau wire buf op' op'' \<Longrightarrow>
-  wstep_comp_op_R io wire buf op op''\<close>
-| \<open>step Tau op op' \<Longrightarrow> wstep_comp_op_R io wire buf op' op'' \<Longrightarrow> wstep_comp_op_R io wire buf op op''\<close>
-
-lemma
-  \<open>wstep io (comp_op wire buf op\<^sub>1 op\<^sub>2) op' \<longleftrightarrow>
-  (\<exists>buf' buf'' buf''' op\<^sub>1' op\<^sub>2'. op' = comp_op wire buf' op\<^sub>1' op\<^sub>2'
-  \<and> wstep_comp_op_L io wire buf'' op\<^sub>1 op\<^sub>1' \<and> wstep_comp_op_R io wire buf''' op\<^sub>2 op\<^sub>2'
-  \<and> (\<forall>p. \<exists>n \<le> length (buf p @ buf'' p). buf' p = drop n (buf p @ buf'' p) \<and> buf''' p = take n (buf p @ buf'' p)))\<close>
-  oops
-
-lemma
-  \<open>wstep io (comp_op (\<lambda>_. None) (\<lambda>_. []) op\<^sub>1 op\<^sub>2) op' \<longleftrightarrow>
-  (\<exists>op\<^sub>1' op\<^sub>2'. op' = comp_op (\<lambda>_. None) (\<lambda>_. []) op\<^sub>1' op\<^sub>2'
-  \<and> wstep_comp_op_L io (\<lambda>_. None) (\<lambda>_. []) op\<^sub>1 op\<^sub>1' \<and> wstep_comp_op_R io (\<lambda>_. None) (\<lambda>_. []) op\<^sub>2 op\<^sub>2')\<close>
-  apply (intro iffI)
-  subgoal
-    sorry
-  subgoal
-    sorry
-  oops
 
 end
